ironfleet/src/Dafny/Distributed/Services/SHT/AppInterface.s.dfy
@@ -4,7 +4,7 @@ abstract module AppInterface_s {
     import opened Native__NativeTypes_s
 
     type Key(==, !new)
-    type Value
+    type Value(==, !new)
 
     predicate method KeyLt(ka:Key, kb:Key) 
 
